lean/privacy/notes/discoverable_outgoing.lean
@@ -10,49 +10,65 @@ theorem ScanOutgoingNoteContext.from {crypto: Crypto} (rm: ReachableMemory crypt
     toScanNoteContext := .from rm,
   }
 
-def scan_outgoing_notes_for_recipient
+def scan_outgoing_notes_for_sender
     {crypto: Crypto} {m: Memory} (context: ScanOutgoingNoteContext crypto m)
     (addralice kalice: ℕ)
-    : List ScannedNote := do
+    : List ExScannedNote := List.dedup <| do
   let addrbob ← scan_outgoing_channels context.toScanOutgoingChannelContext addralice kalice
   let Kbob := m .PublicKeys [addrbob]
   let c := crypto.hash [addralice, kalice, addrbob, Kbob]
   let token ← scan_tokens_for_channel (context.toScanTokenContext) c
-  scan_notes_for_channel context.toScanNoteContext c token
+  let sn ← scan_notes_for_channel context.toScanNoteContext c token
+  return ⟨sn, addralice, addrbob⟩
 
-theorem scan_outgoing_notes_for_recipient_implies
-    {crypto: Crypto} {rm: ReachableMemory crypto} {addralice kalice: ℕ} {sn: ScannedNote} :
-    (h: sn ∈ scan_outgoing_notes_for_recipient (.from rm) addralice kalice) →
-    note_exists rm (sn.note_id crypto) ∧
-    ∃ addrbob kbob, sn.c = crypto.hash [addralice, kalice, addrbob, kbob] := by
-  simp only [scan_outgoing_notes_for_recipient, List.bind_eq_flatMap, List.mem_flatMap]
-  intro h
-  obtain ⟨addrbob, h_bob, token, h_token, h⟩ := h
-  have ⟨h_c, h_token⟩ := scan_notes_for_channel_props h
+theorem NoteImplies.from_scan_outgoing_notes_for_sender
+    {crypto: Crypto} {rm: ReachableMemory crypto} {addralice kalice: ℕ} {esn: ExScannedNote}
+    (h: esn ∈ scan_outgoing_notes_for_sender (.from rm) addralice kalice) :
+    ∃ (inp: CreateNoteInput) (_note_imp: NoteImplies rm inp),
+    inp.to_ex_scanned_note crypto = esn ∧ inp.addralice = addralice ∧ inp.kalice = kalice := by
+  simp only [scan_outgoing_notes_for_sender, List.bind_eq_flatMap, List.mem_dedup, List.mem_flatMap,
+    List.pure_def, List.mem_singleton] at h
+
+  obtain ⟨addrbob, h_bob, token, h_token, sn, h_sn, h_esn⟩ := h
+  have ⟨h_c, h_token⟩ := scan_notes_for_channel_props h_sn
   let Kbob := rm.m MemoryType.PublicKeys [addrbob]
-  refine ⟨?_, ⟨addrbob, Kbob, h_c⟩⟩
 
-  unfold scan_notes_for_channel at h
-  simp only [List.mem_flatMap, List.mem_range] at h
-  obtain ⟨i₀, i₀_lt, h⟩ := h
-  unfold scan_notes_for_channel_i₀ at h
-  simp only [List.mem_map, List.mem_range, Nat.lt_find_iff] at h
-  obtain ⟨i₁, h, h_note_id⟩ := h
+  unfold scan_notes_for_channel at h_sn
+  simp only [List.mem_flatMap, List.mem_range] at h_sn
+  obtain ⟨i₀, i₀_lt, h_sn⟩ := h_sn
+  unfold scan_notes_for_channel_i₀ at h_sn
+  simp only [List.mem_map, List.mem_range, Nat.lt_find_iff] at h_sn
+  obtain ⟨i₁, h_sn, h_note_id⟩ := h_sn
 
-  replace h := h i₁ (by rfl)
-  rw [←h_note_id]
-  exact h
+  replace h_sn := h_sn i₁ (by rfl)
+  rw [h_esn, ←h_note_id]
 
-theorem notes_are_discoverable_outgoing
+  have ⟨inp, note_impl, h_note_id⟩ := NoteImplies.from_note_exists h_sn
+  apply crypto.h_hash at h_note_id
+  injections
+
+  have h_c' : inp.c crypto = crypto.hash [addralice, kalice, addrbob, rm.m MemoryType.PublicKeys [addrbob]] := by assumption
+  apply crypto.h_hash at h_c'
+  injections
+
+  refine ⟨inp, note_impl, ?_, by assumption, by assumption⟩
+  ext
+  all_goals simp [*]
+
+theorem NoteImplies.scan_outgoing
     {crypto: Crypto} {rm: ReachableMemory crypto} {inp: CreateNoteInput}
     (note_imp: NoteImplies rm inp) :
-    inp.to_scanned_note crypto ∈ scan_outgoing_notes_for_recipient (.from rm) inp.addralice inp.kalice := by
+    inp.to_ex_scanned_note crypto ∈ scan_outgoing_notes_for_sender (.from rm) inp.addralice inp.kalice := by
   have := note_imp.subchannel.channel.scan
 
   have h_Kbob := note_imp.subchannel.channel.bob_registered.public_key
   simp only [note_imp.h_Kbob] at h_Kbob
 
-  simp only [scan_outgoing_notes_for_recipient, List.bind_eq_flatMap, List.mem_flatMap]
-  refine ⟨inp.addrbob, ?_, inp.token, h_Kbob ▸ note_imp.subchannel.scan, h_Kbob ▸ note_imp.scan_for_channel⟩
-  rw [note_imp.h_kalice]
-  use outgoing_channels_are_discoverable note_imp.subchannel.channel.h_channel_exists
+  simp only [scan_outgoing_notes_for_sender, List.bind_eq_flatMap, List.mem_dedup, List.mem_flatMap,
+    List.pure_def, List.mem_singleton]
+  refine ⟨inp.addrbob, ?_, inp.token, h_Kbob ▸ note_imp.subchannel.scan, inp.to_scanned_note crypto, ?_, ?_⟩
+  · rw [note_imp.h_kalice]
+    use outgoing_channels_are_discoverable note_imp.subchannel.channel.h_channel_exists
+  · rw [h_Kbob]
+    exact note_imp.scan_for_channel
+  · simp [*]
