lean/privacy/tracing/tracing.lean
@@ -1,0 +1,283 @@
+import privacy.tracing.tracing_context
+import privacy.tracing.graph
+
+def TracingContext.alice {crypto: Crypto} {m: Memory} {events: List Event}
+    (context: TracingContext crypto m events) (coin: Coin crypto m) : UserPrivKey crypto m :=
+  have h := context.h_coin_props_alice coin
+  let kalice: crypto.PrivateKeys := ⟨get_priv_key crypto events coin.esn.addralice, h.1⟩
+  ⟨coin.esn.addralice, kalice, h.2.1⟩
+
+def TracingContext.bob {crypto: Crypto} {m: Memory} {events: List Event}
+    (context: TracingContext crypto m events) (coin: Coin crypto m) : UserPrivKey crypto m :=
+  have h := context.h_coin_props_bob coin
+  let kbob: crypto.PrivateKeys := ⟨get_priv_key crypto events coin.esn.addrbob, h.1⟩
+  ⟨coin.esn.addrbob, kbob, h.2.1⟩
+
+def incoming_equiv_outgoing
+  {crypto: Crypto} {m: Memory} {events: List Event}
+  (context: TracingContext crypto m events)
+  (user: UserPrivKey crypto m) (token: ℕ) :=
+  amounts_to_coins.equiv
+    (ℓ₀ := spent_notes_ex context.toScanNoteContext user.addr user.k token)
+    (ℓ₁ := nonopen_created_notes context.toScanOutgoingNoteContext user.addr user.k token)
+    (h_nodup₀ := by
+      apply List.Nodup.filter
+      apply List.Nodup.filter
+      apply List.nodup_dedup
+    )
+    (h_nodup₁ := by
+      apply List.Nodup.filter
+      apply List.Nodup.filter
+      apply List.nodup_dedup
+    )
+    (f := λ esn ↦ esn.amount crypto m)
+    (g := λ esn ↦ esn.amount crypto m)
+    (h_sum := by rw [context.h_incoming_eq_outgoing])
+
+theorem TracingContext.next_coin_spent_notes_ex {crypto: Crypto} {m: Memory} {events: List Event}
+    (context: TracingContext crypto m events) (coin: Coin crypto m)
+    (h_spent: m MemoryType.Nullifiers [crypto.hash [coin.esn.c, coin.esn.token, coin.esn.i₀, coin.esn.i₁, (context.bob coin).k]] ≠ 0) :
+    let bob := context.bob coin
+    (coin.esn, coin.coin_idx) ∈ (amounts_to_coins
+       (spent_notes_ex context.toScanNoteContext bob.addr bob.k coin.esn.token)
+       (λ esn => esn.amount crypto m)).toFinset := by
+  simp only [List.mem_toFinset, amounts_to_coins.mem]
+  refine ⟨?_, coin.h_coin_idx⟩
+  simp only [spent_notes_ex, List.mem_filter, decide_eq_true_eq, and_true]
+  have h := context.h_coin_props_bob coin
+  refine ⟨h.2.2 h.1, h_spent⟩
+
+def TracingContext.prev_coin_helper {crypto: Crypto} {m: Memory} {events: List Event}
+    (context: TracingContext crypto m events) (coin: Coin crypto m)
+    (h_nonopen: is_open_note crypto m (coin.esn.note_id crypto) = false) :
+    let alice := context.alice coin
+    (coin.esn, coin.coin_idx) ∈ (amounts_to_coins
+       (nonopen_created_notes context.toScanOutgoingNoteContext alice.addr alice.k coin.esn.token)
+       (λ esn => esn.amount crypto m)).toFinset := by
+    simp only [List.mem_toFinset, amounts_to_coins.mem]
+    refine ⟨?_, coin.h_coin_idx⟩
+    simp only [nonopen_created_notes, List.mem_filter, decide_eq_true_eq, and_true]
+    have h := context.h_coin_props_alice coin
+    refine ⟨h.2.2, h_nonopen⟩
+
+def TracingContext.next_coin₀ {crypto: Crypto} {m: Memory} {events: List Event}
+    (context: TracingContext crypto m events) (coin: Coin crypto m)
+    (h_spent: m MemoryType.Nullifiers [crypto.hash [coin.esn.c, coin.esn.token, coin.esn.i₀, coin.esn.i₁, (context.bob coin).k]] ≠ 0) :
+    let bob := context.bob coin
+    { v : ExScannedNote × ℕ // v ∈ (
+      amounts_to_coins
+        (nonopen_created_notes context.toScanOutgoingNoteContext bob.addr bob.k coin.esn.token)
+        (λ esn ↦ esn.amount crypto m)
+      ).toFinset
+    } := by
+  intro bob
+  let incoming_outgoing := incoming_equiv_outgoing context bob coin.esn.token
+  exact incoming_outgoing ⟨⟨coin.esn, coin.coin_idx⟩, context.next_coin_spent_notes_ex _ h_spent⟩
+
+def TracingContext.prev_coin₀ {crypto: Crypto} {m: Memory} {events: List Event}
+    (context: TracingContext crypto m events) (coin: Coin crypto m)
+    (h_nonopen: is_open_note crypto m (coin.esn.note_id crypto) = false) :
+    let alice := context.alice coin
+    { v : ExScannedNote × ℕ // v ∈ (
+      amounts_to_coins
+        (spent_notes_ex context.toScanNoteContext alice.addr alice.k coin.esn.token)
+        (λ esn ↦ esn.amount crypto m)
+      ).toFinset
+    }  := by
+  intro alice
+  let incoming_outgoing := incoming_equiv_outgoing context alice coin.esn.token
+  exact incoming_outgoing.invFun ⟨⟨coin.esn, coin.coin_idx⟩, context.prev_coin_helper _ h_nonopen⟩
+
+theorem TracingContext.next_prev₀
+    {crypto: Crypto} {m: Memory} {events: List Event}
+    (context: TracingContext crypto m events) (coin₀ coin₁: Coin crypto m)
+    (token: ℕ) (h_token₀: token = coin₀.esn.token)
+    (user: UserPrivKey crypto m) (h_user₀: user = context.bob coin₀)
+    (h_spent: m MemoryType.Nullifiers [crypto.hash [coin₀.esn.c, coin₀.esn.token, coin₀.esn.i₀, coin₀.esn.i₁, (context.bob coin₀).k]] ≠ 0)
+    (h_nonopen: is_open_note crypto m (coin₁.esn.note_id crypto) = false) :
+    context.next_coin₀ coin₀ h_spent = (coin₁.esn, coin₁.coin_idx) ↔
+    context.prev_coin₀ coin₁ h_nonopen = (coin₀.esn, coin₀.coin_idx) := by
+  set res₀ := context.next_coin₀ coin₀ h_spent with h_res₀
+  set res₁ := context.prev_coin₀ coin₁ h_nonopen with h_res₁
+  have (a b: Prop): (a ∨ b → (a ↔ b)) → (a ↔ b) := by
+    by_cases h: a; all_goals simp [h]
+  apply this
+  intro h_or
+
+  have ⟨h_addr₁, h_token₁⟩ : coin₀.esn.addrbob = coin₁.esn.addralice ∧ token = coin₁.esn.token := by
+    cases h_or
+    case inl h_or =>
+      have := res₀.prop
+      rw [List.mem_toFinset, amounts_to_coins.mem] at this
+      simp only [nonopen_created_notes, List.mem_filter, decide_eq_true_eq] at this
+      have ⟨h_addralice, Kbob, h_c⟩ := context.h_scan_outgoing_notes_for_sender _ _ _ this.1.1.1
+      simp only [TracingContext.bob, h_or] at h_addralice
+
+      have h_token := this.1.1.2.symm
+      simp only [h_or] at h_token
+
+      exact ⟨h_addralice, h_token₀ ▸ h_token⟩
+    case inr h_or =>
+      have := res₁.prop
+      rw [List.mem_toFinset, amounts_to_coins.mem] at this
+      simp only [spent_notes_ex, List.mem_filter, decide_eq_true_eq] at this
+      have ⟨h_addrbob, kalice, h_c⟩ := context.h_scan_notes_for_recipient (context.alice coin₁) _ this.1.1.1
+      simp only [TracingContext.alice, h_or] at h_addrbob
+
+      have h_token := this.1.1.2.symm
+      simp only [h_or] at h_token
+
+      exact ⟨h_addrbob.symm, h_token₀ ▸ h_token.symm⟩
+
+  replace h_user₁ : user = context.alice coin₁ := by
+    rw [h_user₀]
+    simp only [TracingContext.bob, TracingContext.alice]
+    conv => lhs; arg 1; rw [h_addr₁]
+    conv => lhs; arg 2; arg 1; rw [h_addr₁]
+
+  let incoming_outgoing := incoming_equiv_outgoing context user token
+  have h_res₀' : res₀.1 = (incoming_outgoing ⟨⟨coin₀.esn, coin₀.coin_idx⟩, h_token₀ ▸ h_user₀ ▸ context.next_coin_spent_notes_ex _ h_spent⟩).1 := by
+    cases h_token₀
+    cases h_user₀
+    rfl
+  have h_res₁' : res₁.1 = (incoming_outgoing.symm ⟨⟨coin₁.esn, coin₁.coin_idx⟩, h_token₁ ▸ h_user₁ ▸ context.prev_coin_helper _ h_nonopen⟩).1 := by
+    cases h_token₁
+    cases h_user₁
+    rfl
+
+  rw [h_res₀']
+  have (S: Type) (p q: S → Prop) (e: Equiv { s // p s } { s // q s}) (x y: S) (h_x: p x) (h_y: q y):
+      ↑(e ⟨x, h_x⟩) = y ↔ ↑(e.symm ⟨y, h_y⟩) = x := by
+    have : e ⟨x, h_x⟩ = ⟨y, h_y⟩ ↔ ↑(e ⟨x, h_x⟩) = y := by apply Subtype.ext_iff
+    rw [←this]
+
+    have : e.symm ⟨y, h_y⟩ = ⟨x, h_x⟩ ↔ ↑(e.symm ⟨y, h_y⟩) = x := by apply Subtype.ext_iff
+    rw [←this]
+
+    rw [e.apply_eq_iff_eq_symm_apply]
+    constructor
+    all_goals intro h; rw [h]
+
+  rw [this, h_res₁']
+
+def TracingContext.next_coin₁ {crypto: Crypto} {m: Memory} {events: List Event}
+    (context: TracingContext crypto m events) (coin: Coin crypto m)
+    (h_spent: m MemoryType.Nullifiers [crypto.hash [coin.esn.c, coin.esn.token, coin.esn.i₀, coin.esn.i₁, (context.bob coin).k]] ≠ 0) :
+    Coin crypto m := by
+  let ⟨⟨esn, coin_idx⟩, h_next⟩ := context.next_coin₀ coin h_spent
+
+  simp only [List.mem_toFinset, amounts_to_coins.mem, nonopen_created_notes, List.mem_filter, decide_eq_true_eq] at h_next
+  refine ⟨esn, coin_idx, h_next.2, ?_⟩
+  have ⟨h_addralice, Kbob, h_c⟩ := context.h_scan_outgoing_notes_for_sender _ _ _ h_next.1.1.1
+  use (context.bob coin).k, Kbob, h_c
+
+def TracingContext.prev_coin₁ {crypto: Crypto} {m: Memory} {events: List Event}
+    (context: TracingContext crypto m events) (coin: Coin crypto m)
+    (h_nonopen: is_open_note crypto m (coin.esn.note_id crypto) = false) :
+    Coin crypto m := by
+  let ⟨⟨esn, coin_idx⟩, h_prev⟩ := context.prev_coin₀ coin h_nonopen
+
+  simp only [List.mem_toFinset, amounts_to_coins.mem, spent_notes_ex, List.mem_filter, decide_eq_true_eq] at h_prev
+  refine ⟨esn, coin_idx, h_prev.2, ?_⟩
+  have ⟨h_addrbob, kalice, h_c⟩ := context.h_scan_notes_for_recipient (context.alice coin) _ h_prev.1.1.1
+  use kalice, crypto.priv_to_pub (context.alice coin).k, h_c
+
+theorem TracingContext.next_prev₁
+    {crypto: Crypto} {m: Memory} {events: List Event}
+    (context: TracingContext crypto m events) (coin₀ coin₁: Coin crypto m)
+    (h_spent: m MemoryType.Nullifiers [crypto.hash [coin₀.esn.c, coin₀.esn.token, coin₀.esn.i₀, coin₀.esn.i₁, (context.bob coin₀).k]] ≠ 0)
+    (h_nonopen: is_open_note crypto m (coin₁.esn.note_id crypto) = false) :
+    context.next_coin₁ coin₀ h_spent = coin₁ ↔
+    context.prev_coin₁ coin₁ h_nonopen = coin₀ := by
+  simp only [TracingContext.next_coin₁, TracingContext.prev_coin₁]
+  simp only [Coin.ext_iff]
+  have := context.next_prev₀ coin₀ coin₁ _ (by rfl) _ (by rfl) h_spent h_nonopen
+  simp only [Prod.ext_iff] at this
+  exact this
+
+def TracingContext.next_coin {crypto: Crypto} {m: Memory} {events: List Event}
+  (context: TracingContext crypto m events)
+  (coin: Coin crypto m) : Option (Coin crypto m) := by
+  let bob := context.bob coin
+
+  -- Check if the note was spent.
+  by_cases h_is_spent: m MemoryType.Nullifiers [crypto.hash [coin.esn.c, coin.esn.token, coin.esn.i₀, coin.esn.i₁, bob.k]] ≠ 0
+  case neg => exact none
+
+  exact some (context.next_coin₁ coin h_is_spent)
+
+def TracingContext.prev_coin
+    {crypto: Crypto} {m: Memory} {events: List Event}
+    (context: TracingContext crypto m events)
+    (coin: Coin crypto m) :
+    Option (Coin crypto m) := by
+  let alice := context.alice coin
+
+  -- Check if the note is an open note.
+  by_cases h_nonopen: is_open_note crypto m (coin.esn.note_id crypto)
+  case pos => exact none
+
+  exact some (context.prev_coin₁ coin (by simp only [h_nonopen]))
+
+theorem TracingContext.next_coin_none
+    {crypto: Crypto} {m: Memory} {events: List Event}
+    (context: TracingContext crypto m events)
+    (coin: Coin crypto m) :
+    context.next_coin coin = none ↔
+    m MemoryType.Nullifiers [crypto.hash [coin.esn.c, coin.esn.token, coin.esn.i₀, coin.esn.i₁, (context.bob coin).k]] = 0 := by
+  simp only [TracingContext.next_coin]
+  split_ifs <;> simp [*]; omega
+
+theorem TracingContext.prev_coin_none
+    {crypto: Crypto} {m: Memory} {events: List Event}
+    (context: TracingContext crypto m events)
+    (coin: Coin crypto m) :
+    context.prev_coin coin = none ↔
+    is_open_note crypto m (coin.esn.note_id crypto) := by
+  simp only [TracingContext.prev_coin]
+  split_ifs <;> simp [*]
+
+theorem TracingContext.next_prev
+    {crypto: Crypto} {m: Memory} {events: List Event}
+    (context: TracingContext crypto m events)
+    (coin₀ coin₁: Coin crypto m) :
+    context.next_coin coin₀ = some coin₁ ↔
+    context.prev_coin coin₁ = some coin₀ := by
+  simp only [TracingContext.next_coin, TracingContext.prev_coin]
+  simp only [ne_eq, dite_not, Option.dite_none_left_eq_some, Option.some.injEq, Bool.not_eq_true]
+  constructor
+  · intro ⟨h_spent, h⟩
+    have h_nonopen : is_open_note crypto m (ScannedNote.note_id crypto coin₁.esn.toScannedNote) = false := by
+      rw [←h]
+      simp only [TracingContext.next_coin₁]
+      set res := context.next_coin₀ coin₀ h_spent
+      have := res.prop
+      rw [List.mem_toFinset, amounts_to_coins.mem] at this
+      simp only [nonopen_created_notes, List.mem_filter, decide_eq_true_eq] at this
+      exact this.1.2
+    have := context.next_prev₁ coin₀ coin₁ h_spent h_nonopen
+    use h_nonopen, this.1 h
+  · intro ⟨h_nonopen, h⟩
+    have h_nullifier : m MemoryType.Nullifiers [crypto.hash [coin₀.esn.c, coin₀.esn.token, coin₀.esn.i₀, coin₀.esn.i₁, ↑(context.bob coin₀).k]] ≠ 0 := by
+      rw [←h]
+      simp only [TracingContext.prev_coin₁]
+      set res := context.prev_coin₀ coin₁ h_nonopen
+      have := res.prop
+      rw [List.mem_toFinset, amounts_to_coins.mem] at this
+      simp only [spent_notes_ex, List.mem_filter, decide_eq_true_eq] at this
+      simp only [TracingContext.bob]
+      have h_addr := (context.h_scan_notes_for_recipient (context.alice coin₁) _ this.1.1.1).1
+      rw [←h_addr]
+      exact this.1.2
+    have := context.next_prev₁ coin₀ coin₁ h_nullifier h_nonopen
+    use h_nullifier, this.2 h
+
+def TracingContext.tracing_graph
+    {crypto: Crypto} {m: Memory} {events: List Event}
+    (context: TracingContext crypto m events) :
+    Graph (Coin crypto m) := {
+  next := context.next_coin
+  prev := context.prev_coin,
+  next_iff_prev := by intro coin₀ coin₁; apply TracingContext.next_prev
+  h_fintype := context.h_fintype_coin
+}
