lean/privacy/tracing/tracing_context.lean
@@ -1,0 +1,174 @@
+import privacy.tracing.outgoing_notes
+import privacy.tracing.incoming_notes
+import privacy.tracing.coin
+
+structure TracingContext (crypto: Crypto) (m: Memory) (events: List Event)
+    extends ScanOutgoingNoteContext crypto m where
+  h_incoming_eq_outgoing: ∀ (user: UserPrivKey crypto m) (token: ℕ),
+    (
+      spent_notes_ex toScanNoteContext user.addr user.k token
+      |>.map (λ sn ↦ sn.amount crypto m)
+      |>.sum
+    ) = (
+      nonopen_created_notes toScanOutgoingNoteContext user.addr user.k token
+      |>.map (λ sn ↦ sn.amount crypto m)
+      |>.sum
+    )
+  h_coin_props_alice : ∀ coin: Coin crypto m,
+    let kalice := get_priv_key crypto events coin.esn.addralice
+    kalice ∈ crypto.PrivateKeys ∧
+    m MemoryType.PublicKeys [coin.esn.addralice] = crypto.priv_to_pub kalice ∧
+    coin.esn ∈ scan_outgoing_notes_for_sender toScanOutgoingNoteContext coin.esn.addralice kalice
+  h_coin_props_bob : ∀ coin: Coin crypto m,
+    let kbob := get_priv_key crypto events coin.esn.addrbob
+    kbob ∈ crypto.PrivateKeys ∧
+    m MemoryType.PublicKeys [coin.esn.addrbob] = crypto.priv_to_pub kbob ∧
+    ∀ h, coin.esn ∈ scan_notes_for_recipient toScanNoteContext coin.esn.addrbob ⟨kbob, h⟩
+  h_scan_outgoing_notes_for_sender: ∀ (addralice kalice: ℕ) (esn: ExScannedNote),
+    esn ∈ scan_outgoing_notes_for_sender toScanOutgoingNoteContext addralice kalice →
+    addralice = esn.addralice ∧
+    ∃ Kbob, esn.c = crypto.hash [esn.addralice, kalice, esn.addrbob, Kbob]
+  h_scan_notes_for_recipient: ∀ (bob: UserPrivKey crypto m) (esn: ExScannedNote),
+    esn ∈ scan_notes_for_recipient toScanNoteContext bob.addr bob.k →
+    bob.addr = esn.addrbob ∧
+    ∃ kalice, esn.c = crypto.hash [esn.addralice, kalice, esn.addrbob, crypto.priv_to_pub bob.k]
+  h_fintype_coin: Nonempty (Fintype (Coin crypto m))
+  h_open_note_from_event: ∀ note_id user_enc: ℕ,
+    .CreateOpenNote note_id user_enc ∈ events →
+    is_open_note crypto m note_id
+
+theorem incoming_eq_outgoing
+    {crypto: Crypto} (stxs: SuccessfulTransactions crypto) (user: UserPrivKey crypto stxs.rm.m) (token: ℕ) :
+    (
+      spent_notes_ex (.from stxs.rm) user.addr user.k token
+      |>.map (λ sn ↦ sn.amount crypto stxs.rm)
+      |>.sum
+    ) = (
+      nonopen_created_notes (.from stxs.rm) user.addr user.k token
+      |>.map (λ sn ↦ sn.amount crypto stxs.rm)
+      |>.sum
+    ) := by
+  -- Simplify LHS:
+  set f_amount := (λ sn: ExScannedNote ↦ sn.amount crypto stxs.rm)
+  have : f_amount = (λ sn: ScannedNote ↦ sn.amount crypto stxs.rm) ∘ (λ sn: ExScannedNote ↦ ↑sn) := by rfl
+  conv =>
+    lhs
+    rw [this, ←List.map_map]
+    rw [spent_notes_ex_eq_spent_notes]
+
+  -- Both hands:
+  rw [incoming_notes, outgoing_notes]
+  apply congrArg
+  apply List.map_congr_left
+  intro tx h_tx
+  rw [List.mem_filter] at h_tx
+  rw [←tx.sum_create_note_amounts_eq_nonopen _ h_tx.1, tx.h_balance]
+
+theorem TracingContext.from {crypto: Crypto} (stxs: SuccessfulTransactions crypto) :
+    TracingContext crypto stxs.rm.m stxs.rm.events := {
+  toScanOutgoingNoteContext := .from stxs.rm,
+  h_incoming_eq_outgoing := λ user token ↦ incoming_eq_outgoing stxs user token
+  h_coin_props_alice := by
+    intro coin kalice
+    have ⟨kalice', Kbob, h_c⟩ := coin.h_c
+    have ⟨inp, note_imp, h_note_id⟩ := NoteImplies.from_coin coin
+
+    have h_inp₀ := CreateNoteInput.to_scanned_note_eq h_note_id
+    have h_inp₁ := ScannedNote.ext_iff.1 h_inp₀
+    simp only [h_c] at h_inp₁
+    have h_inp₂ := crypto.h_hash h_inp₁.1
+    injections
+
+    have h_addralice : coin.esn.addralice = inp.addralice := by simp [*]
+
+    have h_public_keys: stxs.rm.m MemoryType.PublicKeys [coin.esn.addralice] = crypto.priv_to_pub inp.kalice := by
+      rw [h_addralice]
+
+      have := note_imp.subchannel.channel.alice_registered.public_key
+      simp only at this
+      exact note_imp.h_kalice ▸ this
+
+    have kalice_priv : inp.kalice ∈ crypto.PrivateKeys :=
+      note_imp.h_kalice ▸ note_imp.subchannel.channel.alice_registered.h_kalice
+
+    have register_imp := RegisterImplies.for_get_priv_key stxs.rm coin.esn.addralice (
+      by rw [h_public_keys]; apply crypto.zero_not_public_key ⟨inp.kalice, kalice_priv⟩)
+
+    refine ⟨?_, ?_, ?_⟩
+    · exact register_imp.h_kalice
+    · rw [register_imp.public_key]
+    · rw [h_addralice]
+
+      have h_kalice : kalice = inp.kalice := by
+        apply crypto.priv_to_pub_inj register_imp.h_kalice kalice_priv
+        rw [←h_public_keys, register_imp.public_key]
+      rw [h_kalice]
+
+      have := note_imp.scan_outgoing
+      simp only at this
+      convert this
+      apply ExScannedNote.ext
+      · simp [h_inp₀]
+      · simp only [h_addralice]
+      · simp [*]
+  h_coin_props_bob := by
+    intro coin kbob
+
+    have ⟨kalice, Kbob, h_c⟩ := coin.h_c
+
+    have ⟨inp, note_imp, h_note_id⟩ := NoteImplies.from_coin coin
+    have h_inp₀ := CreateNoteInput.to_scanned_note_eq h_note_id
+    have h_inp₁ := ScannedNote.ext_iff.1 h_inp₀
+    simp only [h_c] at h_inp₁
+    have h_inp₂ := crypto.h_hash h_inp₁.1
+    injections
+
+    have h_addrbob : coin.esn.addrbob = inp.addrbob := by simp [*]
+
+    have h_public_keys: stxs.rm.m MemoryType.PublicKeys [coin.esn.addrbob] = crypto.priv_to_pub note_imp.subchannel.channel.kbob := by
+      rw [h_addrbob]
+
+      have := note_imp.subchannel.channel.bob_registered.public_key
+      simp only at this
+      exact this
+
+    have register_imp := RegisterImplies.for_get_priv_key stxs.rm coin.esn.addrbob (
+      by rw [h_public_keys]; apply crypto.zero_not_public_key)
+
+    refine ⟨?_, ?_, ?_⟩
+    · exact register_imp.h_kalice
+    · rw [register_imp.public_key]
+    · rw [h_addrbob]
+      intro h
+
+      have h_kbob : ⟨kbob, h⟩ = note_imp.subchannel.channel.kbob := by
+        apply Subtype.coe_inj.1
+        apply crypto.priv_to_pub_inj h (by simp)
+        rw [←h_public_keys, register_imp.public_key]
+      rw [h_kbob]
+
+      have := note_imp.scan_for_recipient
+      simp only at this
+      simp [h_inp₀] at this
+      convert this
+      simp [*]
+  h_scan_outgoing_notes_for_sender := by
+    intro addralice kalice esn h
+    have ⟨inp, note_imp, h_esn, h_addralice, h_kalice⟩ := NoteImplies.from_scan_outgoing_notes_for_sender h
+    rw [←h_esn]
+    refine ⟨by rw [←h_addralice], inp.Kbob, ?_⟩
+    simp only [note_imp.subchannel.h_c, ChannelImplies.c, CreateChannelInput.c, ←h_kalice]
+  h_scan_notes_for_recipient := by
+    intro bob esn h
+    have ⟨inp, note_imp, h_esn, h_addrbob, _, _, _⟩ := NoteImplies.from_scan_notes_for_recipient bob.h_k h
+    rw [←h_esn]
+    refine ⟨by simp [*], inp.kalice, ?_⟩
+    simp only [note_imp.subchannel.h_c, ChannelImplies.c, CreateChannelInput.c, note_imp.h_kalice]
+    simp [*]
+  h_fintype_coin := ⟨Coin.fintype⟩
+  h_open_note_from_event := by
+    intro note_id user_enc h
+    have ⟨inp, note_imp, h_note_id, h_r, _⟩ := NoteImplies.from_open_note_event h
+    have := h_note_id ▸ h_r ▸ note_imp.h_r
+    rw [is_open_note, decide_eq_true_eq, this]
+}
